Finish binding TreeSync and TreeKEM

fstar/new/TreeSyncTreeKEMBinder.fst
@@ -9,7 +9,16 @@ module TK = TreeKEM
 open Lib.Result
 
 //TODO I guess this is somewhere in the standard library
-assume val pub_to_secret: pb:pub_bytes -> b:bytes{Seq.length b == Seq.length pb}
+val pub_to_secret: pb:pub_bytes -> b:bytes{Seq.length b == Seq.length pb}
+let pub_to_secret pb =
+  let open Lib.IntTypes in
+  Seq.seq_of_list (List.Tot.map (fun x -> u8 (v x)) (Seq.seq_to_list pb))
+
+//TODO this shouldn't exist if the rest of the code (parsers, treekem) was written correctly
+val secret_to_pub: b:bytes -> pb:pub_bytes{Seq.length b == Seq.length pb}
+let secret_to_pub b =
+  let open Lib.IntTypes in
+  Seq.seq_of_list (List.Tot.map (fun x -> byte (v x)) (Seq.seq_to_list b))
 
 //TODO They should be the same type
 let dir_ts_to_tk (dir:TS.direction_t) =
@@ -23,12 +32,18 @@ let dir_tk_to_ts (dir:TK.direction) =
 
 let encrypted_path_secret_nt_to_tk (cs:ciphersuite) (x:hpke_ciphertext_nt): result (TK.path_secret_ciphertext cs) =
   if not (Seq.length x.hcn_kem_output = hpke_kem_output_length cs) then
-    fail "kem_output has wrong length"
+    fail "encrypted_path_secret_nt_to_tk: kem_output has wrong length"
   else
-    Success ({
+    return ({
       TK.kem_output = x.hcn_kem_output;
       TK.ciphertext = x.hcn_ciphertext;
     })
+
+let nat_to_index_l (l:nat) (x:nat): result (TK.index_l l) =
+  if not (x < pow2 l) then
+    fail "nat_to_index_l: unmerged leaf index is too big"
+  else
+    return x
 
 val treesync_to_treekem: #l:nat -> cs:ciphersuite -> TS.tree_t l -> result (TK.tree cs l)
 let rec treesync_to_treekem #l cs t =
@@ -51,15 +66,66 @@ let rec treesync_to_treekem #l cs t =
       content <-- from_option "Couldn't parse UpdatePathNode"
         ((ps_to_pse ps_update_path_node).parse_exact (pub_to_secret np.TS.np_content));
       path_secret_ciphertext <-- mapM (encrypted_path_secret_nt_to_tk cs) (Seq.seq_to_list content.upnn_encrypted_path_secret);
+      unmerged_leafs <-- mapM (nat_to_index_l l) (np.TS.np_unmerged_leafs);
       if not (Seq.length content.upnn_public_key = hpke_public_key_length cs) then
         fail ""
       else (
         let kp: TK.key_package cs l = {
           TK.kp_public_key = content.upnn_public_key;
-          TK.unmerged_leafs = admit(); //TODO
+          TK.unmerged_leafs = unmerged_leafs;
           TK.path_secret_from = dir_ts_to_tk (np.TS.np_content_dir);
           TK.path_secret_ciphertext = path_secret_ciphertext;
         } in
-        admit()
+        return (TK.Node (Some kp) tk_left tk_right)
       )
   end
+
+let encrypted_path_secret_tk_to_nt (#cs:ciphersuite) (x:TK.path_secret_ciphertext cs): result (hpke_ciphertext_nt) =
+  if not (Seq.length x.TK.kem_output < pow2 16) then
+    fail "encrypted_path_secret_tk_to_nt: kem_output too long"
+  else if not (Seq.length x.TK.ciphertext < pow2 16) then
+    fail "encrypted_path_secret_tk_to_nt: ciphertext too long"
+  else
+    return ({
+      hcn_kem_output = x.TK.kem_output;
+      hcn_ciphertext = x.TK.ciphertext;
+    })
+
+
+val treekem_to_treesync: #l:nat -> #cs:ciphersuite -> TS.credential_t -> TK.path cs l -> result (TS.path_t l)
+let rec treekem_to_treesync #l #cs cred p =
+  match p with
+  | TK.PLeaf None ->
+    return (TS.PLeaf None)
+  | TK.PLeaf (Some mi) ->
+    return (TS.PLeaf (Some ({
+      TS.lp_credential = {cred with TS.cred_enc_key = secret_to_pub (mi.TK.mi_public_key)};
+      TS.lp_version = 0; //TODO
+    })))
+  | TK.PNode None p_next ->
+    next <-- treekem_to_treesync cred p_next;
+    return (TS.PNode None next)
+  | TK.PNode (Some kp) p_next ->
+    next <-- treekem_to_treesync cred p_next;
+    ciphertexts <-- mapM encrypted_path_secret_tk_to_nt kp.TK.path_secret_ciphertext;
+    //TODO: the two following conditions could be theorems in Crypto
+    if not (1 <= Seq.length kp.TK.kp_public_key) then
+      fail "treekem_to_treesync: public_key too short"
+    else if not (Seq.length kp.TK.kp_public_key < pow2 16) then
+      fail "treekem_to_treesync: public_key too long"
+    else if not (byte_length ps_hpke_ciphertext ciphertexts < pow2 16) then
+      fail "treekem_to_treesync: ciphertexts too long"
+    else begin
+      Seq.lemma_list_seq_bij ciphertexts;
+      let np_content = ps_update_path_node.serialize ({
+        upnn_public_key = kp.TK.kp_public_key;
+        upnn_encrypted_path_secret = Seq.seq_of_list ciphertexts;
+      }) in
+      let np = ({
+        TS.np_version = 0; //TODO
+        TS.np_content_dir = dir_tk_to_ts kp.TK.path_secret_from;
+        TS.np_unmerged_leafs = List.Tot.map (fun (x:TK.index_l l) -> (x<:nat)) kp.TK.unmerged_leafs;
+        TS.np_content = secret_to_pub np_content;
+      }) in
+      return (TS.PNode (Some np) next)
+    end
